coq/model/Consistency1.v
@@ -1,0 +1,13 @@
+From Coq Require Import ZArith List.
+From compcert.lib Require Import Integers Maps.
+From compcert.common Require Import Memory AST.
+From bpf.model Require Import ebpf rBPFCommType rBPFSyntax rBPFDecoder rBPFEncoder.
+
+Import ListNotations.
+
+Lemma rbpf_encode_decode_consistency:
+  forall l_bin pc l ins
+    (HL: list_in_list Int64.eq l_bin pc l = true)
+    (Hencode: rbpf_encoder ins = l_bin),
+      rbpf_decoder pc l = Some ins.
+Admitted.
